ILL_paper_proofs.v
@@ -215,50 +215,50 @@ Module PaperProofsString.
 
 
   Lemma Copy_Proof_from_figure_1:
-  {D, P & 1, R & 1, D ⊸ (((P ⊸ S) ⊕ (R ⊸ (1 ⊕ (P ⊸ S)))) ⊗ D)} ⊢ ((S ⊗ D) ⊕ D).
+    {D, P & 1, R & 1, D ⊸ (((P ⊸ S) ⊕ (R ⊸ (1 ⊕ (P ⊸ S)))) ⊗ D)} ⊢ ((S ⊗ D) ⊕ D).
   Proof with (try solve [id]).
-      impl_l ({D}) ({(P&1) , (R&1) }) (D) ((((P ⊸ S) ⊕ (R ⊸ (1 ⊕ (P ⊸ S)))) ⊗ D))...
-      times_l ((P ⊸ S) ⊕ (R ⊸ (1 ⊕ (P ⊸ S)))) D.
-      oplus_l (P ⊸ S) (R ⊸ (1 ⊕ (P ⊸ S))).
-      - and_l_1 P 1.
-        and_l_2 R 1.
+    impl_l ({D}) ({(P&1) , (R&1) }) D (((P ⊸ S) ⊕ (R ⊸ (1 ⊕ (P ⊸ S)))) ⊗ D)...
+    times_l ((P ⊸ S) ⊕ (R ⊸ (1 ⊕ (P ⊸ S)))) D.
+    oplus_l (P ⊸ S) (R ⊸ (1 ⊕ (P ⊸ S))).
+    - and_l_1 P 1.
+      and_l_2 R 1.
+      one_l.
+      apply Oplus_R_1.
+      times_r ({P, (P ⊸ S) }) ({D})...
+      impl_l  ({P}) (∅) (P) (S)...
+    - and_l_1 R 1.
+      impl_l({R}) ({D, P & 1 }) (R) ((1 ⊕ (P ⊸ S)))...
+      oplus_l 1 (P ⊸ S).
+      + one_l.
+        and_l_2 P 1.
         one_l.
+        apply Oplus_R_2...
+      + and_l_1 (P) 1.
         apply Oplus_R_1.
-        times_r ({P, (P ⊸ S) }) ({D})...
-        impl_l  ({P}) (∅) (P) (S)...
-      - and_l_1 R 1.
-        impl_l({R}) ({D, P & 1 }) (R) ((1 ⊕ (P ⊸ S)))...
-        oplus_l 1 (P ⊸ S).
-        + one_l.
-          and_l_2 P 1.
-          one_l.
-          apply Oplus_R_2...
-        + and_l_1 (P) 1.
-          apply Oplus_R_1.
-          times_r ({ P , P ⊸ S}) ({D})...
-          impl_l ({P}) (∅) (P) (S)...
-    Qed.
+        times_r ({ P , P ⊸ S}) ({D})...
+        impl_l ({P}) (∅) (P) (S)...
+  Qed.
 
   (* Same proof as above but with some more automation *)
   Lemma Copy_Proof_from_figure_1_with_weak_search:
-  {D, P & 1, R & 1, D ⊸ (((P ⊸ S) ⊕ (R ⊸ (1 ⊕ (P ⊸ S)))) ⊗ D)} ⊢ ((S ⊗ D) ⊕ D).
+    {D, P & 1, R & 1, D ⊸ (((P ⊸ S) ⊕ (R ⊸ (1 ⊕ (P ⊸ S)))) ⊗ D)} ⊢ ((S ⊗ D) ⊕ D).
   Proof with try now id.
     impl_l  ({D}) ({(P&1) , (R&1) }) (D) ((((P ⊸ S) ⊕ (R ⊸ (1 ⊕ (P ⊸ S)))) ⊗ D))...
     search_one_goal ({D, (P ⊸ S) ⊕ (R ⊸ (1 ⊕ (P ⊸ S))), P & 1, R & 1} ⊢ (S ⊗ D) ⊕ D).
     oplus_l (P ⊸ S) (R ⊸ (1 ⊕ (P ⊸ S))).
-    search_one_goal ({P, P ⊸ S, D} ⊢ (S ⊗ D) ⊕ D).
-    apply Oplus_R_1.
-    times_r ({P, (P ⊸ S) }) ({D})...
-    impl_l ({P}) (∅) (P) (S)...
-    search_one_goal ({R, R ⊸ (1 ⊕ (P ⊸ S)), D, P & 1} ⊢ (S ⊗ D) ⊕ D).
-    impl_l ({R}) ({D, P & 1 }) (R) ((1 ⊕ (P ⊸ S)))...
-    oplus_l 1 (P ⊸ S).
-    search_one_goal ({D} ⊢ (S ⊗ D) ⊕ D).
-    apply Oplus_R_2...
-    search_one_goal ( {P ⊸ S, D, P} ⊢ (S ⊗ D) ⊕ D).
-    apply Oplus_R_1.
-    times_r ({ P , P ⊸ S}) ({D})...
-    impl_l ({P}) (∅) (P) (S)...
+    - search_one_goal ({P, P ⊸ S, D} ⊢ (S ⊗ D) ⊕ D).
+      apply Oplus_R_1.
+      times_r ({P, (P ⊸ S) }) ({D})...
+      impl_l ({P}) (∅) (P) (S)...
+    - search_one_goal ({R, R ⊸ (1 ⊕ (P ⊸ S)), D, P & 1} ⊢ (S ⊗ D) ⊕ D).
+      impl_l ({R}) ({D, P & 1 }) (R) ((1 ⊕ (P ⊸ S)))...
+      oplus_l 1 (P ⊸ S).
+      + search_one_goal ({D} ⊢ (S ⊗ D) ⊕ D).
+        apply Oplus_R_2...
+      + search_one_goal ( {P ⊸ S, D, P} ⊢ (S ⊗ D) ⊕ D).
+        apply Oplus_R_1.
+        times_r ({ P , P ⊸ S}) ({D})...
+        impl_l ({P}) (∅) (P) (S)...
   Qed.
 
   Lemma Copy_Proof_from_figure_1_with_stronger_search:
@@ -273,86 +273,67 @@ Module PaperProofsString.
       search_one_goal_strong ( {P ⊸ S, D, P} ⊢ (S ⊗ D)).
       times_r  ({ P , P ⊸ S}) ({D})...
   Qed.
-End figure_1.
+  End figure_1.
 
-(** Figure 5 de epsrc_case_for_support. *)
-Section figure_5.
-  Local Notation "'D'" := (Proposition "vD'"%string).
-  Local Notation "'D₁'" := (Proposition "vD1'"%string).
-  Local Notation "'D₀'" := (Proposition "vD0'"%string).
-  Local Notation "'D₂'" := (Proposition "vD2'"%string).
-  Local Notation "'H'" := (Proposition "vH'"%string).
-  Local Notation "'F'":= (Proposition "vF'"%string).
-  Local Notation "'G'" := (Proposition "vG'"%string).
-  Local Notation "'M'" := (Proposition "vM'"%string).
-  Local Notation "'L'" := (Proposition "vL'"%string).
+  (** Figure 5 de epsrc_case_for_support. *)
+  Section figure_5.
+    Local Notation "'D'" := (Proposition "vD'"%string).
+    Local Notation "'D₁'" := (Proposition "vD1'"%string).
+    Local Notation "'D₀'" := (Proposition "vD0'"%string).
+    Local Notation "'D₂'" := (Proposition "vD2'"%string).
+    Local Notation "'H'" := (Proposition "vH'"%string).
+    Local Notation "'F'":= (Proposition "vF'"%string).
+    Local Notation "'G'" := (Proposition "vG'"%string).
+    Local Notation "'M'" := (Proposition "vM'"%string).
+    Local Notation "'L'" := (Proposition "vL'"%string).
 
 
-  Local Notation "'ρ'" := ({ H,F,L,D₂, G⊸(!(H⊸(H⊗M))) }).
-  Local Notation "'μ'" := ({ !((D₁⊗M)⊸D₀),!((D₂⊗M)⊸D₁)}).
-  Local Notation "'λ'" := ({ !((L⊗D₀)⊸(L⊗D₁)),!((L⊗D₁)⊸(L⊗D₂))}).
+    Local Notation "'ρ'" := ({ H,F,L,D₂, G⊸(!(H⊸(H⊗M))) }).
+    Local Notation "'μ'" := ({ !((D₁⊗M)⊸D₀),!((D₂⊗M)⊸D₁)}).
+    Local Notation "'λ'" := ({ !((L⊗D₀)⊸(L⊗D₁)),!((L⊗D₁)⊸(L⊗D₂))}).
 
-  (* Ltac bang_c  p'   :=  *)
-  (*   match goal with  *)
-  (*     |- ILL_proof ?env _ => *)
-  (*       match env with *)
-  (*         | context C [(!p'::?env')] => *)
-  (*           let e := context C [ env' ] in   *)
-  (*             with_multiset (!p'::e) ltac:(apply Bang_C) *)
-  (*       end *)
-  (*   end. *)
-
-  (* Ltac bang_d  p'   :=  *)
-  (*   match goal with  *)
-  (*     |- ILL_proof ?env _ => *)
-  (*       match env with *)
-  (*         | context C [(!p'::?env')] => *)
-  (*           let e := context C [ env' ] in   *)
-  (*             with_multiset (!p'::e) ltac:(apply Bang_D) *)
-  (*       end *)
-  (*   end. *)
-
-  Lemma figure_5 : 
-    {H,L,G,D₂,G⊸!(H⊸(H⊗M)),(L⊗(D₂⊗H))⊸(L⊗(D₀⊗((L⊗D₂)⊸D)))}∪λ∪μ⊢D.
-  Proof with try now (finish_proof_strong || prove_multiset_eq).
-      search_one_goal_strong ({H,L,D₂,!(H⊸(H⊗M)),(L⊗(D₂⊗H))⊸(L⊗(D₀⊗((L⊗D₂)⊸D)))}∪λ∪μ⊢D).
+    Lemma figure_5 : 
+      {H,L,G,D₂,G⊸!(H⊸(H⊗M)),(L⊗(D₂⊗H))⊸(L⊗(D₀⊗((L⊗D₂)⊸D)))}∪λ∪μ⊢D.
+    Proof with try now (finish_proof_strong || prove_multiset_eq).
+      search_one_goal_strong ({H, L, D₂, ! (H ⊸ H ⊗ M),(L⊗(D₂⊗H))⊸(L⊗(D₀⊗((L⊗D₂)⊸D)))}∪λ∪μ⊢D).
       bang_c (H⊸(H⊗M)).
       bang_d ((H⊸(H⊗M))).
-      search_one_goal_strong ((H ⊗ M)
-        :: {L, D₂, !(H ⊸ (H ⊗ M)),
-          (L ⊗ (D₂ ⊗ H)) ⊸ (L ⊗ (D₀ ⊗ ((L ⊗ D₂) ⊸ D)))} ∪ 
-        λ ∪ μ⊢D).
-      search_one_goal_strong ( {H ,M,L, D₂, !(H ⊸ (H ⊗ M)),
-        (L ⊗ (D₂ ⊗ H)) ⊸ (L ⊗ (D₀ ⊗ ((L ⊗ D₂) ⊸ D)))} ∪ 
-      λ ∪ μ⊢D).
+      search_one_goal_strong
+        ((H ⊗ M) ::
+           {L, D₂, !(H ⊸ (H ⊗ M)), (L ⊗ (D₂ ⊗ H)) ⊸ (L ⊗ (D₀ ⊗ ((L ⊗ D₂) ⊸ D)))}
+           ∪ λ ∪ μ⊢D).
+      search_one_goal_strong
+        ({H ,M,L, D₂, !(H ⊸ (H ⊗ M)),
+            (L ⊗ (D₂ ⊗ H)) ⊸ (L ⊗ (D₀ ⊗ ((L ⊗ D₂) ⊸ D)))}
+           ∪ λ ∪ μ⊢D).
       bang_c ((D₂⊗M)⊸D₁).
       bang_d ((D₂⊗M)⊸D₁).
-      impl_l ({M,D₂}) ({H, L,  !(H ⊸ (H ⊗ M)), (L ⊗ (D₂ ⊗ H)) ⊸ (L ⊗ (D₀ ⊗ ((L ⊗ D₂) ⊸ D)))} ∪ λ ∪ μ) (D₂⊗M) (D₁).
-      times_r ({ D₂}) ({M})...
-      search_one_goal_strong ({D₁,H, L,  (L ⊗ (D₂ ⊗ H)) ⊸ (L ⊗ (D₀ ⊗ ((L ⊗ D₂) ⊸ D)))} ∪ λ ⊢ D).
-      bang_c ((L⊗D₁)⊸(L⊗D₂))...
-      bang_d ((L⊗D₁)⊸(L⊗D₂))...
-      impl_l ({L,D₁}) ({H, (L ⊗ (D₂ ⊗ H)) ⊸ (L ⊗ (D₀ ⊗ ((L ⊗ D₂) ⊸ D)))}∪λ) (L⊗D₁) (L⊗D₂)...
-      times_r  ({L}) ({D₁})...
-      search_one_goal_strong ({L,D₂,H, (L ⊗ (D₂ ⊗ H)) ⊸ (L ⊗ (D₀ ⊗ ((L ⊗ D₂) ⊸ D)))} ∪ λ ⊢ D).
-      impl_l ({L,D₂,H}) ({ !((L⊗D₀)⊸(L⊗D₁)),!((L⊗D₁)⊸(L⊗D₂))}) (L⊗(D₂⊗H)) ((L ⊗ (D₀ ⊗ ((L ⊗ D₂) ⊸ D))))...
-      times_r ({L}) ({D₂,H})...
-      times_r ({D₂}) ({H})...
-      search_one_goal_strong ({L,D₀,((L ⊗ D₂) ⊸ D)}∪λ⊢D).
-      bang_c ((L⊗D₀)⊸(L⊗D₁))...
-      bang_d ((L⊗D₀)⊸(L⊗D₁))...
-      impl_l 
-        ({L,D₀})
-        ({!((L ⊗ D₀) ⊸ (L ⊗ D₁)), (L ⊗ D₂) ⊸ D, !((L ⊗ D₁) ⊸ (L ⊗ D₂))})
-        (L⊗D₀)
-        (L⊗D₁)...
-      times_r ({L}) ({D₀})...
-      search_one_goal_strong (   {L ⊗ D₁, (L ⊗ D₂) ⊸ D, !((L ⊗ D₁) ⊸ (L ⊗ D₂))} ⊢ D).
-      bang_c 
-      (((L ⊗ D₁) ⊸ (L ⊗ D₂)))...
-      bang_d 
-        (((L ⊗ D₁) ⊸ (L ⊗ D₂)))...
-Qed.
+      impl_l ({M,D₂}) ({H, L,  !(H ⊸ (H ⊗ M)), (L ⊗ (D₂ ⊗ H)) ⊸ (L ⊗ (D₀ ⊗ ((L ⊗ D₂) ⊸ D)))}
+                         ∪ λ ∪ μ) (D₂⊗M) (D₁).
+      - times_r ({ D₂}) ({M})...
+      - search_one_goal_strong ({D₁,H, L,  (L ⊗ (D₂ ⊗ H)) ⊸ (L ⊗ (D₀ ⊗ ((L ⊗ D₂) ⊸ D)))} ∪ λ ⊢ D).
+        bang_c ((L⊗D₁)⊸(L⊗D₂))...
+        bang_d ((L⊗D₁)⊸(L⊗D₂))...
+        impl_l ({L,D₁}) ({H, (L ⊗ (D₂ ⊗ H)) ⊸ (L ⊗ (D₀ ⊗ ((L ⊗ D₂) ⊸ D)))}∪λ) (L⊗D₁) (L⊗D₂)...
+        + times_r  ({L}) ({D₁})...
+        + search_one_goal_strong ({L,D₂,H, (L ⊗ (D₂ ⊗ H)) ⊸ (L ⊗ (D₀ ⊗ ((L ⊗ D₂) ⊸ D)))} ∪ λ ⊢ D).
+          impl_l ({L,D₂,H}) ({ !((L⊗D₀)⊸(L⊗D₁)),!((L⊗D₁)⊸(L⊗D₂))}) (L⊗(D₂⊗H))
+            ((L ⊗ (D₀ ⊗ ((L ⊗ D₂) ⊸ D))))...
+          * times_r ({L}) ({D₂,H})...
+            times_r ({D₂}) ({H})...
+          * search_one_goal_strong ({L,D₀,((L ⊗ D₂) ⊸ D)}∪λ⊢D).
+            bang_c ((L⊗D₀)⊸(L⊗D₁))...
+            bang_d ((L⊗D₀)⊸(L⊗D₁))...
+            impl_l 
+              ({L,D₀})
+                ({!((L ⊗ D₀) ⊸ (L ⊗ D₁)), (L ⊗ D₂) ⊸ D, !((L ⊗ D₁) ⊸ (L ⊗ D₂))})
+                (L⊗D₀)
+                (L⊗D₁)...
+            -- times_r ({L}) ({D₀})...
+            -- search_one_goal_strong ({L ⊗ D₁, (L ⊗ D₂) ⊸ D, !((L ⊗ D₁) ⊸ (L ⊗ D₂))} ⊢ D).
+               bang_c ((L ⊗ D₁) ⊸ (L ⊗ D₂))...
+               bang_d ((L ⊗ D₁) ⊸ (L ⊗ D₂))...
+    Qed.
 
-End figure_5.
+  End figure_5.
 End PaperProofsString.
