emma_orig.v
@@ -7,30 +7,29 @@ Open Scope ILL_scope.
 
 (* Declaration of basic propositions. *)
 Declare Scope Emma.
-Notation "'P'" := (Proposition 1%nat):Emma. (* Poison *)
+Notation "'P'" := (Proposition 1%nat):Emma. (* Emma take the Poison *)
 Notation "'R'" := (Proposition 2%nat):Emma. (* discussion with Rodolph *)
 Notation "'G'" := (Proposition 3%nat):Emma. (* discussion with Guillaumin *)
 Notation "'B'" := (Proposition 4%nat):Emma. (* discussion with Binet *)
-Notation "'V'" := (Proposition 5%nat) (only parsing):Emma.
-Notation "'S'" := (Proposition 5%nat):Emma.
-Notation "'A'" := (Proposition 6%nat):Emma.
-Notation "'E'" := (Proposition 7%nat):Emma.
-Notation "'M'" := (Proposition 8%nat):Emma.
+Notation "'S'" := (Proposition 5%nat):Emma. (* Emma sells herself *)
+Notation "'E'" := (Proposition 7%nat):Emma. (* Emma and Rodolphe Escape together *)
+Notation "'A'" := (Proposition 6%nat):Emma. (* Emma stay Alive *)
+Notation "'D'" := (Proposition 8%nat):Emma. (* Emma dies (Meurt) *)
 
 
 Open Scope ILL_scope.
 Open Scope Emma.
 
-Lemma simpl_ex: {P ⊸ M, P, !(S ⊸ A)} ⊢ A ⊕ M.
+Lemma simpl_ex: {P ⊸ D, P, !(S ⊸ A)} ⊢ A ⊕ D.
 Proof with try solve [ apply Id;reflexivity | prove_multiset_eq].
-  bang_w (S ⊸ A)...
-  weak_impl_l P M...
+  bang_w (S ⊸ A).
+  weak_impl_l P D...
   apply Oplus_R_2...
 Defined.
 
 (* EXAMPLE OF IMPOSSIBLE INTERNAL CHOICE *)
 Lemma originelle :
-  {P&1, R, G, B&1, !(S⊸A), (E⊸A)&1, (P⊸M)&1,(R⊸1)&(R⊸E), (G⊸1)⊕(G⊸S), 1⊕((B⊸S)&(B⊸1))  } ⊢ A ⊕ M .
+  {P&1, R, G, B&1, !(S⊸A), (E⊸A)&1, (P⊸D)&1,(R⊸1)&(R⊸E), (G⊸1)⊕(G⊸S), 1⊕((B⊸S)&(B⊸1))  } ⊢ A ⊕ D .
 Proof with try solve [ apply Id;reflexivity | prove_multiset_eq].
   and_l_2 (R⊸1) (R⊸E).
   oplus_l (G ⊸ 1) (G ⊸ S).
@@ -45,7 +44,7 @@ Proof with try solve [ apply Id;reflexivity | prove_multiset_eq].
 Abort.
 
 Lemma originelle :
-  {P&1, R, G, B&1, !(S⊸A), (E⊸A)&1, (P⊸M)&1,(R⊸1)&(R⊸E), (G⊸1)⊕(G⊸S), 1⊕((B⊸S)&(B⊸1))  } ⊢ A ⊕ M .
+  {P&1, R, G, B&1, !(S⊸A), (E⊸A)&1, (P⊸D)&1,(R⊸1)&(R⊸E), (G⊸1)⊕(G⊸S), 1⊕((B⊸S)&(B⊸1))  } ⊢ A ⊕ D .
 Proof with try solve [ apply Id;reflexivity | prove_multiset_eq].
   oplus_l (G ⊸ 1) (G ⊸ S).
   - (* Left branch *)
@@ -62,17 +61,17 @@ Proof with try solve [ apply Id;reflexivity | prove_multiset_eq].
       weak_impl_l R 1...
       and_l_1 P 1.
       and_l_2 (E ⊸ A) 1.
-      and_l_1 (P ⊸ M) 1.
+      and_l_1 (P ⊸ D) 1.
       do 2 one_l.
       bang_w (S ⊸ A)...
-      weak_impl_l P M...
+      weak_impl_l P D...
       apply Oplus_R_2...
     + (* Left right *)
       and_l_2 B 1.
       do 2 one_l.
       and_l_2 P 1.
       and_l_1 (E ⊸ A) 1.
-      and_l_2 (P ⊸ M) 1.
+      and_l_2 (P ⊸ D) 1.
       and_l_2 (R ⊸ 1) (R ⊸ E).
       do 2 one_l.
       bang_w (S ⊸ A)...
@@ -89,7 +88,7 @@ Proof with try solve [ apply Id;reflexivity | prove_multiset_eq].
       and_l_2 P 1.
       and_l_2 B 1.
       and_l_2 (E ⊸ A)  1.
-      and_l_2 (P ⊸ M) 1.
+      and_l_2 (P ⊸ D) 1.
       repeat one_l.
       bang_d (S ⊸ A)... (* !D instead of WL *)
       weak_impl_l S A...
@@ -101,7 +100,7 @@ Proof with try solve [ apply Id;reflexivity | prove_multiset_eq].
       one_l.
       and_l_2 P 1.
       and_l_2 (E ⊸ A) 1.
-      and_l_2 (P ⊸ M) 1.
+      and_l_2 (P ⊸ D) 1.
       repeat one_l.
       bang_d (S ⊸ A)... (* !D instead of WL *)
       weak_impl_l S A...
@@ -155,7 +154,7 @@ Ltac search_goal n g :=
 
 
 Lemma originelle' :
-  {P&1, R, G, B&1, !(S⊸A), (E⊸A)&1, (P⊸M)&1,(R⊸1)&(R⊸E), (G⊸1)⊕(G⊸S), 1⊕((B⊸S)&(B⊸1))  } ⊢ A ⊕ M .
+  {P&1, R, G, B&1, !(S⊸A), (E⊸A)&1, (P⊸D)&1,(R⊸1)&(R⊸E), (G⊸1)⊕(G⊸S), 1⊕((B⊸S)&(B⊸1))  } ⊢ A ⊕ D .
 Proof with try solve [ apply Id;reflexivity | prove_multiset_eq].
   oplus_l (G ⊸ 1) (G ⊸ S).
   - weak_impl_l G 1...
@@ -165,7 +164,7 @@ Proof with try solve [ apply Id;reflexivity | prove_multiset_eq].
       do 2 one_l.
       and_l_2 P 1.
       and_l_1 (E ⊸ A) 1.
-      Time search_goal 6 ({R ⊸ E, E ⊸ A, R} ⊢ A ⊕ M).
+      Time search_goal 6 ({R ⊸ E, E ⊸ A, R} ⊢ A ⊕ D).
       finish_proof_strong.
     + and_l_2 (B ⊸ S) (B ⊸ 1).
       and_l_1 B 1.
@@ -174,19 +173,19 @@ Proof with try solve [ apply Id;reflexivity | prove_multiset_eq].
       and_l_1 (R ⊸ 1) (R ⊸ E).
       weak_impl_l R 1...
       and_l_1 P 1.
-      Time search_goal 6 ({P ⊸ M, P} ⊢ A ⊕ M).
+      Time search_goal 6 ({P ⊸ D, P} ⊢ A ⊕ D).
       finish_proof_strong.
   - weak_impl_l G S...
     and_l_1(R ⊸ 1) (R ⊸ E).
     weak_impl_l R 1...
     one_l.
     oplus_l 1 ((B ⊸ S) & (B ⊸ 1)).
-    + search_goal 10 ({S, !(S ⊸ A)} ⊢ A ⊕ M).
+    + search_goal 10 ({S, !(S ⊸ A)} ⊢ A ⊕ D).
       bang_d (S ⊸ A)... (* !D instead of WL *)
       finish_proof_strong.
     + and_l_2 (B ⊸ S) (B ⊸ 1).
       and_l_1 B 1.
-      Time search_goal 10 ({S, !(S ⊸ A)} ⊢ A ⊕ M).
+      Time search_goal 10 ({S, !(S ⊸ A)} ⊢ A ⊕ D).
       bang_d (S ⊸ A)... (* !D instead of WL *)
       finish_proof_strong.
   Qed.
@@ -194,7 +193,7 @@ Proof with try solve [ apply Id;reflexivity | prove_multiset_eq].
 
 (*
 Lemma originelle2 :
-  {P&1, R, G, B&1, !(S⊸A), (E⊸A)&1, (P⊸M)&1,(R⊸1)&(R⊸E), (G⊸1)⊕(G⊸S), 1⊕((B⊸S)&(B⊸1))  } ⊢ A ⊕ M .
+  {P&1, R, G, B&1, !(S⊸A), (E⊸A)&1, (P⊸D)&1,(R⊸1)&(R⊸E), (G⊸1)⊕(G⊸S), 1⊕((B⊸S)&(B⊸1))  } ⊢ A ⊕ D .
 
   and_l_2 (R⊸1) (R⊸E).
 *)
